code/ecdsap256/Hacl.Impl.P384.LowLevel.fst
@@ -24,6 +24,16 @@ open FStar.Tactics.Canon
 open Lib.IntTypes.Intrinsics
 
 
+val mul_p384: f: felem P384 -> r: felem P384 -> out: widefelem P384 -> 
+  Stack unit
+    (requires fun h -> live h out /\ live h f /\ live h r /\ disjoint r out)
+    (ensures  fun h0 _ h1 -> modifies (loc out) h0 h1 /\ 
+      wide_as_nat P384 h1 out = as_nat P384 h0 r * as_nat P384 h0 f
+    )
+
+let mul_p384 f r out = admit()
+
+
 val square_p384: f: felem P384 -> out: widefelem P384 -> Stack unit
     (requires fun h -> live h out /\ live h f /\ eq_or_disjoint f out)
     (ensures  fun h0 _ h1 -> modifies (loc out) h0 h1 /\ wide_as_nat P384 h1 out = as_nat P384 h0 f * as_nat P384 h0 f)
