code/ecdsap256/Hacl.Impl.ECDSA.MM.Exponent.fst
@@ -11,7 +11,7 @@ open Lib.Buffer
 open FStar.Math.Lemmas
 open Hacl.Impl.P256.Math 
 
-open Hacl.Impl.P256.LowLevel 
+open Hacl.Impl.P.LowLevel 
 open Hacl.Lemmas.P256
 open FStar.Tactics
 open FStar.Tactics.Canon 
