code/ecdsap256/Hacl.Impl.P.LowLevel.fsti
@@ -1,0 +1,254 @@
+module Hacl.Impl.P.LowLevel
+
+open FStar.HyperStack.All
+open FStar.HyperStack
+module ST = FStar.HyperStack.ST
+
+open Lib.IntTypes
+open Lib.Buffer
+
+open Hacl.Spec.P256.Definition
+open Hacl.Lemmas.P256
+(* open Spec.ECDSA.Lemmas *)
+open Spec.P256
+open Spec.ECDSA
+
+open FStar.Math
+open FStar.Math.Lemmas
+open FStar.Mul
+
+open FStar.Tactics
+open FStar.Tactics.Canon 
+
+(* open Spec.P256.Lemmas *)
+open Lib.IntTypes.Intrinsics
+
+open Hacl.Impl.P256.LowLevel
+open Hacl.Impl.P384.LowLevel
+
+open Hacl.Spec.P256.MontgomeryMultiplication
+
+
+
+
+val uploadZeroImpl: #c: curve -> f: felem c -> Stack unit 
+  (requires fun h -> live h f)
+  (ensures fun h0 _ h1 -> as_nat c h1 f == 0 /\ modifies (loc f) h0 h1)
+
+
+val uploadZeroPoint: #c: curve -> p: point c -> 
+  Stack unit
+    (requires fun h -> live h p)
+    (ensures fun h0 _ h1 ->     
+      modifies (loc p) h0 h1 /\
+      as_nat P256 h1 (gsub p (size 0) (size 4)) == 0 /\ 
+      as_nat P256 h1 (gsub p (size 4) (size 4)) == 0 /\
+      as_nat P256 h1 (gsub p (size 8) (size 4)) == 0) 
+
+
+
+
+val cmovznz4: #c: curve -> cin: uint64 -> x: felem c -> y: felem c -> result: felem c ->
+  Stack unit
+    (requires fun h -> live h x /\ live h y /\ live h result /\ disjoint x result /\ eq_or_disjoint y result)
+    (ensures fun h0 _ h1 -> modifies1 result h0 h1 /\ 
+      (if uint_v cin = 0 then as_nat c h1 result == as_nat c h0 x else as_nat c h1 result == as_nat c  h0 y))
+
+
+
+val sub_felem: #c: curve -> x: felem c -> y: glbuffer uint64 (getCoordinateLenU64 c) -> result: felem c -> 
+  Stack uint64
+    (requires fun h -> live h x /\ live h y /\ live h result /\ disjoint x result /\ disjoint y result)
+    (ensures fun h0 r h1 -> modifies (loc result) h0 h1 /\ 
+      as_nat c h1 result - v r * pow2 256 == as_nat c h0 x  - as_nat_il c h0 y /\
+      (
+	if uint_v r = 0 then 
+	  as_nat c h0 x >= as_nat_il c h0 y 
+	else 
+	  as_nat c h0 x < as_nat_il c h0 y)
+      )
+
+
+
+val uploadOneImpl: #c: curve -> f: felem c -> Stack unit
+  (requires fun h -> live h f)
+  (ensures fun h0 _ h1 -> as_nat c h1 f == 1 /\ modifies (loc f) h0 h1)
+
+
+
+val toUint8P256: i: felem P256 -> o: lbuffer uint8 (getScalarLen P256) -> Stack unit
+  (requires fun h -> live h i /\ live h o /\ disjoint i o)
+  (ensures fun h0 _ h1 -> modifies (loc o) h0 h1)
+
+
+
+
+val toUint8P384: i: felem P384 -> o: lbuffer uint8 (getScalarLen P384) -> Stack unit
+  (requires fun h -> live h i /\ live h o /\ disjoint i o)
+  (ensures fun h0 _ h1 -> modifies (loc o) h0 h1)
+
+
+
+
+
+  val toUint8: #c: curve -> i: felem c ->  o: lbuffer uint8 (getScalarLen c) -> Stack unit
+  (requires fun h -> live h i /\ live h o /\ disjoint i o)
+  (ensures fun h0 _ h1 -> 
+    modifies (loc o) h0 h1 (*/\ 
+    as_seq h1 o == Lib.ByteSequence.uints_to_bytes_be #_ #_ #4 (as_seq h0 i)  *)
+  )
+
+
+
+val changeEndian: #c: curve -> i: felem c -> Stack unit 
+  (requires fun h -> live h i)
+  (ensures  fun h0 _ h1 -> modifies1 i h0 h1 (*/\ 
+    as_seq h1 i == Hacl.Spec.ECDSA.Definition.changeEndian (as_seq h0 i) /\
+    as_nat P256 h1 i < pow2 256
+  *)  ) 
+
+
+
+val toUint64ChangeEndianP256: i: lbuffer uint8 (size 32) -> o: felem P256 -> 
+  Stack unit
+  (requires fun h -> live h i /\ live h o /\ disjoint i o)
+  (ensures  fun h0 _ h1 -> modifies (loc o) h0 h1)
+
+
+
+val toUint64ChangeEndianP384: i: lbuffer uint8 (size 48) -> o: felem P384 -> 
+  Stack unit
+  (requires fun h -> live h i /\ live h o /\ disjoint i o)
+  (ensures  fun h0 _ h1 -> modifies (loc o) h0 h1)
+
+
+
+
+val toUint64ChangeEndian: #c: curve -> i:lbuffer uint8 (getScalarLen c) -> o: felem c -> Stack unit
+  (requires fun h -> live h i /\ live h o /\ disjoint i o)
+  (ensures  fun h0 _ h1 ->
+    modifies (loc o) h0 h1 (* /\
+    as_seq h1 o == Hacl.Spec.ECDSA.Definition.changeEndian (Lib.ByteSequence.uints_from_bytes_be (as_seq h0 i)) *)
+  )
+
+
+
+
+inline_for_extraction
+let prime256_buffer: x: glbuffer uint64 4ul {witnessed #uint64 #(size 4) x (Lib.Sequence.of_list p256_prime_list) /\ recallable x /\ felem_seq_as_nat P256 (Lib.Sequence.of_list (p256_prime_list)) == prime256} = 
+  assert_norm (felem_seq_as_nat P256 (Lib.Sequence.of_list (p256_prime_list)) == prime256);
+  createL_global p256_prime_list
+
+
+inline_for_extraction
+let prime384_buffer: x: glbuffer uint64 6ul {witnessed #uint64 #(size 6) x (Lib.Sequence.of_list
+p384_prime_list) /\ recallable x /\ felem_seq_as_nat P384 (Lib.Sequence.of_list (p384_prime_list)) == prime384}  = 
+  assert_norm (felem_seq_as_nat P384 (Lib.Sequence.of_list (p384_prime_list)) == prime384);
+  createL_global p384_prime_list
+
+
+inline_for_extraction
+let prime_buffer (#c: curve): (x: glbuffer uint64 (getCoordinateLenU64 c) {witnessed #uint64 #(getCoordinateLenU64 c) x (Lib.Sequence.of_list (prime_list c)) /\ recallable x /\ felem_seq_as_nat c (Lib.Sequence.of_list (prime_list c)) == getPrime c}) = 
+  match c with
+  | P256 -> prime256_buffer
+  | P384 -> prime384_buffer
+
+
+val reduction_prime_2prime_with_carry: #c: curve -> x: widefelem c -> result: felem c -> 
+  Stack unit 
+    (requires fun h -> 
+      live h x /\ live h result /\ eq_or_disjoint x result /\ wide_as_nat c h x < 2 * getPrime c)
+    (ensures fun h0 _ h1 -> 
+      modifies (loc result) h0 h1 /\ as_nat c h1 result = wide_as_nat c h0 x % getPrime c)
+
+
+val reduction_prime_2prime: #c: curve -> x: felem c -> result: felem c -> 
+  Stack unit
+    (requires fun h -> 
+      live h x /\ live h result /\ eq_or_disjoint x result)
+    (ensures fun h0 _ h1 -> 
+      modifies (loc result) h0 h1 /\ as_nat c h1 result == as_nat c h0 x % getPrime c)
+
+
+val felem_add: #c: curve -> a: felem c -> b: felem c -> out: felem c -> 
+  Stack unit
+    (requires (fun h0 -> 
+      live h0 a /\ live h0 b /\ live h0 out /\ eq_or_disjoint a out /\  eq_or_disjoint b out /\
+      as_nat c h0 a < getPrime c /\ as_nat c h0 b < getPrime c 
+      )
+    )
+    (ensures (fun h0 _ h1 -> 
+      modifies (loc out) h0 h1 /\ 
+      as_nat c h1 out == (as_nat c h0 a + as_nat c h0 b) % getPrime c /\
+      as_nat c h1 out == toDomain_ #c((fromDomain_ #c (as_nat c h0 a) + fromDomain_ #c (as_nat c h0 b)) % getPrime c)
+	)
+    )
+
+
+val felem_double: #c: curve -> a: felem c -> out: felem c -> 
+  Stack unit 
+    (requires (fun h0 -> 
+      live h0 a /\ live h0 out /\ eq_or_disjoint a out /\ as_nat c h0 a < getPrime c))
+    (ensures (fun h0 _ h1 -> 
+      modifies (loc out) h0 h1 /\ 
+      as_nat c h1 out == (2 * as_nat c h0 a) % getPrime c /\
+      as_nat c h1 out == toDomain_ #c (2 * fromDomain_ #c (as_nat c h0 a) % getPrime c)
+    )
+  )
+
+
+val felem_sub: #c: curve -> a: felem c -> b: felem c -> out: felem c -> 
+  Stack unit 
+    (requires (fun h0 -> 
+      live h0 out /\ live h0 a /\ live h0 b /\ eq_or_disjoint a out /\ eq_or_disjoint b out /\ 
+      as_nat c h0 a < getPrime c /\ as_nat c h0 b < getPrime c
+      )
+    )
+    (ensures (fun h0 _ h1 -> 
+      modifies (loc out) h0 h1 /\ 
+      as_nat c h1 out == (as_nat c h0 a - as_nat c h0 b) % getPrime c /\
+      as_nat c h1 out == toDomain_ #c ((fromDomain_ #c (as_nat c h0 a) - fromDomain_ #c (as_nat c h0 b)) % getPrime c)
+      )
+    )    
+
+
+
+inline_for_extraction noextract
+val mul: #c: curve -> f: felem c -> r: felem c -> out: widefelem c -> 
+  Stack unit
+    (requires fun h -> live h out /\ live h f /\ live h r /\ disjoint r out)
+    (ensures  fun h0 _ h1 -> modifies (loc out) h0 h1 /\ 
+      wide_as_nat c h1 out = as_nat c h0 r * as_nat c h0 f
+    )
+
+
+
+  
+val eq0_u64: a: uint64 -> Tot (r: uint64 {if uint_v a = 0 then uint_v r == pow2 64 - 1 else uint_v r == 0})
+
+val eq1_u64: a: uint64 -> Tot (r: uint64 {if uint_v a = 0 then uint_v r == 0 else uint_v r == pow2 64 - 1})
+
+
+val isZero_uint64_CT: #c: curve ->  f: felem c -> Stack uint64
+  (requires fun h -> live h f)
+  (ensures fun h0 r h1 -> modifies0 h0 h1 /\ 
+    (if as_nat c h0 f = 0 then uint_v r == pow2 64 - 1 else uint_v r == 0))
+ 
+
+
+ val compare_felem: #c: curve -> a: felem c -> b: felem c -> Stack uint64
+  (requires fun h -> live h a /\ live h b) 
+  (ensures fun h0 r h1 -> modifies0 h0 h1 /\ (if as_nat c h0 a = as_nat c h0 b then uint_v r == pow2 64 - 1 else uint_v r = 0))
+
+
+val copy_conditional: #c: curve -> out: felem c -> x: felem c 
+  -> mask: uint64 {uint_v mask = 0 \/ uint_v mask = pow2 64 - 1} -> Stack unit 
+  (requires fun h -> live h out /\ live h x)
+  (ensures fun h0 _ h1 -> modifies (loc out) h0 h1 /\ 
+    (if uint_v mask = 0 then as_seq h1 out == as_seq h0 out else as_seq h1 out == as_seq h0 x)) 
+
+
+val shiftLeftWord: #c: curve -> i: felem c -> o: lbuffer uint64 (getCoordinateLenU64 c *. 2ul)-> 
+  Stack unit 
+    (requires fun h -> live h i /\ live h o /\ disjoint i o)
+    (ensures fun h0 _ h1 -> modifies1 o h0 h1 /\ wide_as_nat c h1 o == as_nat c h0 i * getPower2 c)
