code/ecdsap256/Hacl.Impl.P256.PointDouble.fst
@@ -13,8 +13,7 @@ open Hacl.Lemmas.P256
 open Hacl.Spec.P256.Definition
 open Hacl.Impl.SolinasReduction
 open Hacl.Spec.P256.MontgomeryMultiplication
-open Hacl.Impl.P256.LowLevel 
-open Hacl.Impl.P256.LowLevel.PrimeSpecific
+open Hacl.Impl.P.LowLevel
 open Hacl.Impl.P256.MontgomeryMultiplication
 open Spec.P256
 open Hacl.Impl.P256.Math 
