code/ecdsap256/Hacl.Impl.P256.PointDouble.fsti
@@ -12,8 +12,8 @@ open Lib.Buffer
 open Hacl.Spec.P256.Definition
 open Hacl.Spec.P256.MontgomeryMultiplication
 open Spec.P256
-open Hacl.Impl.P256.LowLevel 
-open Hacl.Impl.P256.LowLevel.PrimeSpecific
+
+open Hacl.Impl.P.LowLevel 
 open Hacl.Impl.P256.MontgomeryMultiplication
 open Hacl.Impl.P256.Math 
 
